HKDOT: Revise experiments, start w/ indexed judgments

theories/misc_unused/hoInterps_experiments.v
@@ -40,7 +40,7 @@ End try1.
 From D Require Import saved_interp_dep lty asubst_base.
 
 (* *)
-Module simple.
+Module noDepTypes.
 Module Type HoSemTypes (Import VS : VlSortsFullSig) (Import LWP : LiftWp VS).
 Include Lty VS LWP.
 Section saved_dep_use.
@@ -92,17 +92,10 @@ Section saved_dep_use.
   Qed.
 End saved_dep_use.
 End HoSemTypes.
-End simple.
+End noDepTypes.
 
-Module Type HoSemTypes (Import VS : VlSortsFullSig) (Import LWP : LiftWp VS).
-Include Lty VS LWP.
-
-(* XXX Good names? *)
-Notation iPred T Σ := (T → iProp Σ).
-Notation iPredO T Σ := (T -d> iPropO Σ).
-
+Module Type HoSemTypes (Import VS : VlSortsFullSig) (Import LWP : LiftWp VS) (Import L : Lty VS LWP).
 Section saved_ho_sem_type_extra.
-  (* Context `{!savedHoSemTypeG Σ}. *)
   Context {Σ : gFunctors}.
 
   Implicit Types (Ψ : packedHoEnvD Σ).
@@ -134,94 +127,98 @@ Section saved_ho_sem_type_extra.
     unpack Ψ2 a b c.
   Proof. exact: unpack_ne. Qed.
 
-  (** The semantics of a kind includes a predicate on types, and a subtype predicate.
-   *)
-  (* XXX make these non-expansive. *)
-  Definition skind Σ n := env → olty Σ n → iProp Σ.
-  Definition srelkind Σ n := env → olty Σ n → olty Σ n → iProp Σ.
-
-  (* Semantic Full Kind. *)
-  Record sfkind Σ n := Sfkind {
-    sfkind_car :> skind Σ n;
-    sfkind_sub :> srelkind Σ n;
-  }.
-  Global Arguments Sfkind {_ _} _ _.
-  Global Arguments sfkind_car {_ _} _ _ _ : simpl never.
-  Global Arguments sfkind_sub {_ _} _ _ _ _ : simpl never.
-
-  (* Definition app {n} (F : sfkind Σ n) (A : hoD Σ n) := F A. *)
-  Definition app1 {n} (F : sfkind Σ n) : skind Σ n := F.
-  Definition app2 {n} (F : sfkind Σ n) : srelkind Σ n := F.
-
-  Definition subtype {n} : srelkind Σ n := λ ρ (φ1 φ2 : olty Σ n),
-    (□ ∀ (args : vec vl n) v, ⌜ nclosed_vl v 0 ⌝ →
-      φ1 args ρ v → φ2 args ρ v)%I.
-  Definition semEquiv {n} : srelkind Σ n := λ ρ (φ1 φ2 : olty Σ n),
-    (□ ∀ (args : vec vl n) v, ⌜ nclosed_vl v 0 ⌝ →
-      φ1 args ρ v ↔ φ2 args ρ v)%I.
-
-  Notation D := (iPred vl Σ).
-
-  Definition kind_star_subtype1 : srelkind Σ 0 := subtype.
-  Definition kind_star_subtype : srelkind Σ 0 := λ ρ φ1 φ2,
-    (□ ∀ v, ⌜ nclosed_vl v 0 ⌝ → oClose φ1 ρ v → oClose φ2 ρ v)%I.
-  Definition kind_star_eqtype : srelkind Σ 0 := λ ρ φ1 φ2,
-    (□ ∀ v, ⌜ nclosed_vl v 0 ⌝ → oClose φ1 ρ v ↔ oClose φ2 ρ v)%I.
-
-  Lemma kind_star_subtype_eq ρ φ1 φ2 :
-    kind_star_subtype1 ρ φ1 φ2 ≡ kind_star_subtype ρ φ1 φ2.
-  Proof.
-    rewrite /kind_star_subtype1 /kind_star_subtype /subtype /vclose.
-    apply intuitionistically_proper, equiv_spec; split. by iIntros "H".
-    iIntros "H" (args). by rewrite (vec_vnil args).
-  Qed.
-
-  Definition ocurry {n} (Φ : olty Σ (S n)) : vl -d> oltyO Σ n :=
+  Definition oCurry {n} (Φ : olty Σ (S n)) : vl -d> oltyO Σ n :=
     λ v, Olty (λ args, vcurry (oApp Φ) v args).
 
-  Definition ouncurry {n} (Φ : vl -d> oltyO Σ n) : olty Σ (S n) :=
+  Definition oUncurry {n} (Φ : vl -d> oltyO Σ n) : olty Σ (S n) :=
     Olty (λ args, vuncurry Φ args).
+  Definition oLaterN {n} i (τ : olty Σ n) := Olty (eLater i τ).
+End saved_ho_sem_type_extra.
 
-  Definition oclose (φ : olty Σ 0) : env → iPred vl Σ := oClose φ.
+(** The semantics of a kind includes a predicate on types, and a subtype predicate.
+  *)
+(* XXX make these non-expansive? *)
+Notation skind Σ n := (env → olty Σ n → iProp Σ).
+Notation srelkind Σ n := (env → olty Σ n → olty Σ n → iProp Σ).
+
+(* Semantic Full Kind. *)
+Record sfkind Σ n := Sfkind {
+  sfkind_car :> skind Σ n;
+  sfkind_sub : srelkind Σ n;
+}.
+Global Arguments Sfkind {_ _} _ _.
+Global Arguments sfkind_car {_ _} _ _ _ : simpl never.
+Global Arguments sfkind_sub {_ _} _ _ _ _ : simpl never.
+
+(** Kinded, indexed subtyping *)
+Definition sstpk `{dlangG Σ} {n} i j Γ T1 T2 (K : sfkind Σ n) : iProp Σ :=
+  □∀ ρ, s⟦Γ⟧*ρ → sfkind_sub K ρ (oLaterN i T1) (oLaterN j T2).
+(* :: is at level 60. *)
+(* Notation "Γ s⊨k T1 , i <: T2 , j ∷ K" := (sstpk i j Γ T1 T2 K)
+  (at level 74, i, j at level 59, T1, T2, i at next level). *)
+Notation "Γ s⊨ T1 , i <: T2 , j ∷ K" := (sstpk i j Γ T1 T2 K)
+  (at level 74, i, j, T1, T2 at next level).
+
+(* XXX Should we delay [T] as well? Yes, based on [iSel_Sub]/[iSub_Sel].
+Should we delay K?*)
+(* V1: delay K and rely on swaps to make that affect all types. *)
+Definition sktp `{dlangG Σ} {n} i Γ T (K : sfkind Σ n) : iProp Σ :=
+  □∀ ρ, s⟦Γ⟧*ρ → ▷^i K ρ T.
+(* V2: push the delay down. *)
+(* Definition sktp `{dlangG Σ} {n} i Γ T (K : sfkind Σ n) : iProp Σ :=
+  □∀ ρ, s⟦Γ⟧*ρ → K i ρ (oLaterN i T). *)
+(* XXX What delays are wanted here? *)
+Definition ssktp `{dlangG Σ} {n} i Γ (K1 K2 : sfkind Σ n) : iProp Σ :=
+  □∀ ρ τ, s⟦Γ⟧*ρ → ▷^i K1 ρ τ → ▷^i K2 ρ τ.
+
+End HoSemTypes.
+
+From D.Dot Require Import dot_lty unary_lr.
+Module HkDot.
+Include HoSemTypes VlSorts dlang_inst dot_lty.
+
+Section semkinds.
+  Context `{dlangG Σ}.
+
+  Definition subtype {n} : srelkind Σ n := λI ρ (φ1 φ2 : olty Σ n),
+    □ ∀ args v, φ1 args ρ v → φ2 args ρ v.
+
+  Definition skstar : skind Σ 0 := λI ρ φ, True.
+  Definition srstar : srelkind Σ 0 := λ ρ φ1 φ2,
+    (□ ∀ v, oClose φ1 ρ v → oClose φ2 ρ v)%I.
+  Definition sstar : sfkind Σ 0 := Sfkind skstar srstar.
+
+  (* Show that kinded subtyping correctly generalizes the existing kind-*
+  subtyping. *)
+  Lemma sstpk_star_eq_sstp Γ i j T1 T2 :
+    Γ s⊨ T1 , i <: T2 , j ∷ sstar ⊣⊢ Γ s⊨ T1 , i <: T2 , j.
+  Proof.
+    rewrite /sstpk /sfkind_sub/= /srstar; iSplit; iIntros "/= #Hsub !>" (ρ).
+    by iIntros (v) "#Hg"; iApply ("Hsub" $! ρ with "Hg").
+    by iIntros "#Hg" (v) "!>"; iApply ("Hsub" $! ρ v with "Hg").
+  Qed.
 
   Definition skpi {n} (φArg : olty Σ 0) (K : skind Σ n) : skind Σ (S n) :=
-    λI ρ φ, □∀ arg, oClose φArg ρ arg → K ρ (ocurry φ arg).
-
-  (* A possible sketch of kinded subtyping for lambdas? *)
+    λI ρ φ, □∀ arg, oClose φArg ρ arg → K ρ (oCurry φ arg).
   Definition srpi {n} (φArg : olty Σ 0) (Kr : srelkind Σ n) : srelkind Σ (S n) :=
-    λI ρ φ1 φ2, □∀ arg, oClose φArg ρ arg → Kr ρ (ocurry φ1 arg) (ocurry φ2 arg).
-
+    λI ρ φ1 φ2, □∀ arg, oClose φArg ρ arg → Kr ρ (oCurry φ1 arg) (oCurry φ2 arg).
   Definition spi {n} (φArg : olty Σ 0) (K : sfkind Σ n) : sfkind Σ (S n) :=
     Sfkind (skpi φArg (sfkind_car K)) (srpi φArg (sfkind_sub K)).
 
   Definition fold_srelkind (base : srelkind Σ 0) : ∀ n, vec (olty Σ 0) n → srelkind Σ n :=
     vec_fold base (@srpi).
   Definition subtype_w_expKind : ∀ n, vec (olty Σ 0) n → srelkind Σ n :=
-    fold_srelkind kind_star_subtype.
-  Definition eqtype_w_expKind : ∀ n, vec (olty Σ 0) n → srelkind Σ n :=
-    fold_srelkind kind_star_eqtype.
+    fold_srelkind srstar.
+  (* Definition eqtype_w_expKind : ∀ n, vec (olty Σ 0) n → srelkind Σ n :=
+    fold_srelkind kind_star_eqtype. *)
 
   (* The point of Sandro's kind syntax is to use this only at kind 0. *)
   (* Definition sktmem {n} (φ1 φ2 : hoD Σ n) φ :=
     (subtype n 1 1 φ1 φ ∧ subtype n 1 1 φ φ)%I. *)
   Definition skintv (φ1 φ2 : olty Σ 0) : skind Σ 0 := λI ρ φ,
-    subtype ρ φ1 φ ∧ subtype ρ φ φ2.
+    subtype ρ (oLaterN 1 φ1) φ ∧ subtype ρ φ (oLaterN 1 φ2).
   Definition sintv (φ1 φ2 : olty Σ 0) : sfkind Σ 0 :=
-    Sfkind (skintv φ1 φ2) kind_star_subtype.
-  (* Next Obligation.  move=>????? Heq. f_equiv. exact: Heq. solve_proper_ho. *)
-
-  Definition oLaterN {n} i (τ : olty Σ n) := Olty (eLater i τ).
-  Definition skLaterN {n} i (K : skind Σ n) : skind Σ n :=
-    λ ρ φ, K ρ (oLaterN i φ).
-  Definition sfLaterN {n} i (K : sfkind Σ n) : sfkind Σ n :=
-    Sfkind (skLaterN i K) K.
-
-  Definition sktmem (φ1 φ2 : olty Σ 0) : skind Σ 0 :=
-    skLaterN 1 (skintv (oLaterN 1 φ1) (oLaterN 1 φ2)).
-
-  (* Inductive kind : nat → Type :=
-    | kintv : ty → ty → kind 0
-    | kpi n : ty → kind n → kind (S n). *)
+    Sfkind (skintv φ1 φ2) srstar.
 
   Inductive kind {Σ} : nat → Type :=
     | kintv : olty Σ 0 → olty Σ 0 → kind 0
@@ -234,64 +231,128 @@ Section saved_ho_sem_type_extra.
       | kpi n φ1 k' => skpi φ1 (sem k')
     end.
 
+  (* Notice the argument type is not used here. *)
   Inductive hoSTy {Σ} : nat → Type :=
-    | TSWrap : hoEnvD Σ 0 → hoSTy 0
-    | TSLam n : hoEnvD Σ 0 → hoSTy n → hoSTy (S n)
-    | TSApp n : hoSTy (S n) → vl → hoSTy n.
+    | TSWrap : olty Σ 0 → hoSTy 0
+    | TSLam {n} : olty Σ 0 → hoSTy n → hoSTy (S n)
+    | TSApp {n} : hoSTy (S n) → path → hoSTy n.
 
-  Fixpoint hoSTySem {n} (T : hoSTy n): hoEnvD Σ n :=
+  Definition oLam {n} (τ : olty Σ n) : olty Σ (S n) :=
+    oUncurry (λ v, τ.|[v/]).
+    (* Alternatives: *)
+    (* oUncurry (λ v args ρ, τ args (v .: ρ)). *)
+    (* Olty (λ args ρ, τ (vtail args) (vhead args .: ρ)). *)
+  Definition oTApp {n} (τ : olty Σ (S n)) v : olty Σ n := oCurry τ v.
+  Definition oTAppP {n} (τ : olty Σ (S n)) (p : path) : olty Σ n :=
+    Olty (λ args ρ v, path_wp p.|[ρ] (λ w, oCurry τ w args ρ v)).
+
+  Lemma swap_oLam_oLater {n} (τ : olty Σ n) :
+    oLater (oLam τ) ≡ oLam (oLater τ).
+  Proof. done. Qed.
+
+  Lemma swap_oTApp_oLater {n} (τ : olty Σ (S n)) v:
+    oLater (oTApp τ v) ≡ oTApp (oLater τ) v.
+  Proof. done. Qed.
+
+  Fixpoint hoSTySem {n} (T : hoSTy n): olty Σ n :=
     match T with
     | TSWrap φ => φ
-    | TSLam n' φ T =>
-      vuncurry (λ v, (hoSTySem T).|[v/])
-      (* Alternatives: *)
-      (* vuncurry (A := envD Σ) (λ v args ρ, hoSTySem T args (v .: ρ)) *)
-      (* λ args ρ, hoSTySem T (vtail args) (vhead args .: ρ) *)
-    | TSApp n' T v =>
-      vcurry (hoSTySem T) v
+    | TSLam _ T => oLam (hoSTySem T)
+    | TSApp T p => oTAppP (hoSTySem T) p
     end.
-End saved_ho_sem_type_extra.
+End semkinds.
 Arguments hoSTy: clear implicits.
-End HoSemTypes.
+End HkDot.
 
-Module Type HoGenExperimnents (Import VS : VlSortsFullSig) (Import LWP : LiftWp VS).
-Include HoSemTypes VS LWP.
-Include TyInterpLemmas VS LWP.
-Export ty_interp_lemmas.
+From D Require swap_later_impl.
+(* These are "bad" experiments. *)
+Module HoGenExperimnents.
+Import swap_later_impl HkDot.
 Section sec.
-  Context `{TyInterp ty Σ}.
+  Context `{!CTyInterp Σ}.
+  Context `{dlangG Σ} `{HswapProp: SwapPropI Σ}.
+
+  Definition srstar1 : srelkind Σ 0 := subtype.
+  Lemma srstar_eq ρ φ1 φ2 :
+    srstar1 ρ φ1 φ2 ≡ srstar ρ φ1 φ2.
+  Proof.
+    rewrite /srstar1 /srstar /subtype /vclose.
+    apply intuitionistically_proper, equiv_spec; split. by iIntros "H".
+    iIntros "H" (args). by rewrite (vec_vnil args).
+  Qed.
+
+  (* Definition skLaterN {Σ n} i (K : skind Σ n) : skind Σ n :=
+    λ ρ φ, K ρ (oLaterN i φ). *)
+  (* Definition srLaterN {Σ n} i j (K : srelkind Σ n) : srelkind Σ n :=
+    λ ρ T1 T2, K ρ (oLaterN i T1) (oLaterN j T2). *)
+  (* Definition sfLaterN {n} i (K : sfkind Σ n) : sfkind Σ n :=
+    Sfkind (skLaterN i K) K. *)
+
+  (* Definition sstpk `{dlangG Σ} {n} i j Γ τ₁ τ₂ (K : sfkind Σ n) : iProp Σ :=
+    □∀ ρ, s⟦Γ⟧*ρ → srLaterN i j (sfkind_sub K) ρ τ₁ τ₂. *)
+  (* Definition semEquiv {n} : srelkind Σ n := λI ρ (φ1 φ2 : olty Σ n),
+    □ ∀ args v, φ1 args ρ v ↔ φ2 args ρ v. *)
+  (* Definition kind_star_eqtype : srelkind Σ 0 := λ ρ φ1 φ2,
+    (□ ∀ v, oClose φ1 ρ v ↔ oClose φ2 ρ v)%I. *)
+
+
+  Definition sstpk1 {n} i Γ T1 T2 (K : sfkind Σ n) : iProp Σ :=
+    □∀ ρ, s⟦Γ⟧*ρ → ▷^i sfkind_sub K ρ T1 T2.
+  Lemma sstpk1_star_eq_sstp Γ i T1 T2 :
+    sstpk1 i Γ T1 T2 sstar ⊣⊢ Γ s⊨ T1 , i <: T2 , i.
+  Proof using HswapProp.
+    rewrite /sstpk1 /sfkind_sub/= /srstar.
+    iSplit; iIntros "/= #Hsub !>" (ρ); [iIntros (v)|]; iIntros "#Hg".
+    iSpecialize ("Hsub" $! ρ with "Hg"); iSpecialize ("Hsub" $! v).
+    rewrite -mlaterN_pers laterN_impl.
+    by iApply "Hsub".
+    rewrite -mlaterN_pers; iIntros (v) "!>"; rewrite -mlaterN_impl.
+    iDestruct "Hsub" as "#Hsub".
+    iApply ("Hsub" $! ρ v with "Hg").
+  Qed.
+
+  (* Inductive kind : nat → Type :=
+    | kintv : ty → ty → kind 0
+    | kpi n : ty → kind n → kind (S n). *)
+
 
   Inductive htype : nat → Type :=
     | TWrap : ty → htype 0
-    | TLam n : hoEnvD Σ 0 → htype n → htype (S n)
-    | TApp n : htype (S n) → vl → htype n.
+    | TLam {n} : olty Σ 0 → htype n → htype (S n)
+    | TApp {n} : htype (S n) → path → htype n.
 
   Fixpoint htype_to_hosty {n} (T : htype n) : hoSTy Σ n :=
     match T with
-    | TWrap T' => TSWrap (vopen ⟦ T' ⟧)
-    | TLam n' φ T' => TSLam n' φ (htype_to_hosty T')
-    | TApp n' T' v => TSApp n' (htype_to_hosty T') v
+    | TWrap T => TSWrap V⟦T⟧
+    | TLam φ T => TSLam φ (htype_to_hosty T)
+    | TApp T v => TSApp (htype_to_hosty T) v
     end.
   Definition typeSem {n} (T : htype n) : hoEnvD Σ n := hoSTySem (htype_to_hosty T).
 
   Lemma K_App_Lam {n} (argT : olty Σ 0) (φ1 φ2: olty Σ (S n)) (K : srelkind Σ n) ρ :
-    srpi argT K ρ φ1 φ2 ⊣⊢ (□∀ v, oclose argT ρ v → K ρ (ocurry φ1 v) (ocurry φ2 v))%I.
+    srpi argT K ρ φ1 φ2 ⊣⊢ (□∀ v, oClose argT ρ v → K ρ (oCurry φ1 v) (oCurry φ2 v))%I.
   Proof. done. Qed.
   (** XXX Need a subtyping judgment to throw in environments... *)
 
   (* Here, we inherit eta from the metalanguage, in both directions. *)
   (* Er, let's please carry it closer to the syntax? *)
-  Lemma eta1 {n} argT (φ : olty Σ (S n)) ρ : srpi argT subtype ρ φ (ouncurry (ocurry φ)).
+  Lemma eta1 {n} argT (φ : olty Σ (S n)) ρ : srpi argT subtype ρ φ (oUncurry (oCurry φ)).
   Proof.
     rewrite /srpi /subtype.
-    iIntros "!> * #Harg !>" (args v Hcl) "$".
+    iIntros "!> * #Harg !>" (args v) "$".
   Qed.
 
-  Lemma eta {n} argT (φ : olty Σ (S n)) ρ : srpi argT semEquiv ρ φ (ouncurry (ocurry φ)).
+  Lemma eta2 {n} argT (φ : olty Σ (S n)) ρ : srpi argT subtype ρ (oUncurry (oCurry φ)) φ.
+  Proof.
+    rewrite /srpi /subtype.
+    iIntros "!> * #Harg !>" (args v) "$".
+  Qed.
+
+  (* Lemma eta {n} argT (φ : olty Σ (S n)) ρ : srpi argT semEquiv ρ φ (oUncurry (oCurry φ)).
   Proof.
     rewrite /srpi /semEquiv.
     iIntros "!> * #Harg !> **". rewrite -(iff_refl emp%I). done.
-  Qed.
+  Qed. *)
 
   Program Fixpoint sem_program {n} {struct n} : kind Σ n → skind Σ n :=
     match n return _ with
@@ -320,27 +381,24 @@ Section sec.
 End sec.
 End HoGenExperimnents.
 
-From D.Dot Require syn dlang_inst.
-
 Module dot_experiments.
-Import syn dlang_inst.
-Include HoSemTypes VlSorts dlang_inst.
-Include TyInterpLemmas VlSorts dlang_inst.
-Export ty_interp_lemmas.
+Import HkDot.
+(* Include TyInterpLemmas VlSorts dlang_inst.
+Export ty_interp_lemmas. *)
 
 Section sec.
-  Context `{!savedHoSemTypeG Σ} `{!dlangG Σ} `{TyInterp ty Σ}.
-  (* Implicit Types (interp : envD Σ) (φ : D). *)
+  Context `{!savedHoSemTypeG Σ} `{!dlangG Σ} `{CTyInterp Σ}.
 
   Definition dm_to_type (d : dm) n (ψ : hoD Σ n) : iProp Σ :=
     (∃ s σ, ⌜ d = dtysem σ s ⌝ ∧ s ↗n[ σ, n ] ψ)%I.
   Notation "d ↗n[ n ] φ" := (dm_to_type d n φ) (at level 20).
   Global Arguments dm_to_type: simpl never.
 
-  (* Definition def_interp_tmem {n} : skind Σ n → envPred dm Σ :=
-    λ K ρ d, (∃ φ, d.|[ρ] ↗n[ n ] φ ∧ K ρ (Olty φ))%I.
-  Definition def_interp_tmem_spec (φ1 φ2 : hoD Σ 0) : envPred dm Σ :=
-    def_interp_tmem (sktmem φ1 φ2). *)
+  (* [K]'s argument must ignore [ρ]. Patch the definition of skind instead. *)
+  Definition def_interp_tmem {n} (K : skind Σ n): envPred dm Σ :=
+    λI ρ d, ∃ φ, d.|[ρ] ↗n[ n ] φ ∧ K ρ (Olty (λ args ρ v, □ φ args v)).
+  Definition def_interp_tmem_spec (φ1 φ2 : olty Σ 0) : envPred dm Σ :=
+    def_interp_tmem (skintv φ1 φ2).
 End sec.
 
 Notation "d ↗n[ n ] φ" := (dm_to_type d n φ) (at level 20).
